theories/eris/lib/sampling/bernoulli/interface.v
@@ -1,96 +1,89 @@
 From clutch.eris Require Import eris.
 From clutch.eris.lib.sampling Require Import utils.
-From clutch.eris.lib.sampling.bernoulli.tape Require Import interface.
-
 
 #[local] Open Scope R.
 
-Module Type BernoulliSpec (T : BernoulliTapeSpec).
-  Import T.
+Class bernoulli_spec `{!erisGS Σ} (bernoulli_prog : val) :=
+  BernoulliSpec {
+      
+      twp_bernoulli_scale :
+      ∀ (N M : nat) (ε ε1 ε2 : R) 
+        (p := N / S M),
+        N ≤ S M →
+        0 <= ε1 →
+        0 <= ε2 →
+        ε1 * (1 - p) + ε2 * p = ε →
+        [[{↯ ε}]]
+          bernoulli_prog #() #N #M
+          [[{
+                (k : nat), RET #k;
+                (⌜k = 0%nat⌝ ∗ ↯ ε1) ∨
+                  (⌜k = 1%nat⌝ ∗ ↯ ε2)
+          }]];
+
+  bernoulli_case :
+      ∀ (N M : nat),
+        (*TODO: See to add N <= S M  *)
+        [[{True}]]
+          bernoulli_prog #() #N #M
+          [[{v, RET v; ⌜v = #0⌝ ∨ ⌜v = #1⌝}]];
+
+  own_bernoulli_tape :
+      loc → nat → nat → list (fin 2) → iPropI Σ;
+  
+  twp_presample_bernoulli : 
+      ∀ (e : expr) (α : loc) (Φ : val → iProp Σ) 
+        (N M : nat) (ns : list (fin 2)),
+        to_val e = None →
+        own_bernoulli_tape α N M ns ∗ 
+        (∀ i : fin 2, 
+           own_bernoulli_tape α N M (ns ++ [i]) -∗ WP e [{ v, Φ v }]) 
+        ⊢ WP e [{ v, Φ v }];
+  
+  twp_presample_bernoulli_adv_comp : 
+      ∀ (e : expr) (α : loc) (Φ : val → iProp Σ) 
+        (N M : nat) (ns : list (fin 2)) (ε : R) (D : fin 2 → R),
+        N ≤ M + 1 →
+        (∀ i : fin 2, 0 <= D i) →
+        D 0%fin * (1 - N / (M + 1)) + D 1%fin * (N / (M + 1)) = ε →
+        to_val e = None → 
+        own_bernoulli_tape α N M ns ∗ 
+        ↯ ε ∗ 
+        (∀ i : fin 2, 
+           ↯ (D i) ∗ own_bernoulli_tape α N M (ns ++ [i]) -∗ 
+           WP e [{ v, Φ v }])
+        ⊢ WP e [{ v, Φ v }];
+
+  twp_bernoulli_tape :
+      ∀ (N M : nat) (α : loc) (ns : list (fin 2)) (n : fin 2),
+        [[{ own_bernoulli_tape α N M (n::ns) }]]
+          bernoulli_prog (#lbl:α) #N #M
+          [[{ RET #n ; own_bernoulli_tape α N M ns }]];
+      
+      twp_presample_bernoulli_planner :
+      ∀ (N M : nat) (e : expr) (ε : nonnegreal) (L : nat) 
+        (α : loc) (Φ : val → iProp Σ) (prefix : list (fin 2)) 
+        (suffix : list (fin 2) → list (fin 2)),
+        (0 < N < S M)%nat →
+        to_val e = None →
+        (∀ junk : list (fin 2), 
+           (0 < length (suffix (prefix ++ junk)) <= L)%nat) → 
+        0 < ε → 
+        ↯ ε ∗ 
+        own_bernoulli_tape α N M prefix ∗
+        ((∃ junk : list (fin 2), 
+      own_bernoulli_tape α N M (prefix ++ junk ++ suffix (prefix ++ junk))) 
+         -∗ WP e [{ v, Φ v }])
+        ⊢ WP e [{ v, Φ v }]
+    }.
+
+Set Default Proof Using "Type*".
+
+Section BernoulliSpecLemmas.
 
   Context `{!erisGS Σ}.
-
-  Parameter bernoulli_tape : val.
-
-  Notation bernoulli := (bernoulli_tape #())%E.
-
-  Parameter twp_bernoulli_scale :
-    ∀ (N M : nat) (ε ε1 ε2 : R) 
-      (p := N / S M),
-    N ≤ S M →
-    0 <= ε1 →
-    0 <= ε2 →
-    ε1 * (1 - p) + ε2 * p = ε →
-    [[{↯ ε}]]
-      bernoulli #N #M
-    [[{
-      (k : nat), RET #k;
-      (⌜k = 0%nat⌝ ∗ ↯ ε1) ∨
-      (⌜k = 1%nat⌝ ∗ ↯ ε2)
-    }]].
-
-  Parameter bernoulli_spec :
-    ∀ (N M : nat),
-     (*TODO: See to add N <= S M  *)
-    [[{True}]]
-      bernoulli #N #M
-    [[{v, RET v; ⌜v = #0⌝ ∨ ⌜v = #1⌝}]]
-  .
-
-  (* TODO: See to add to a different module ? *)
-  Parameter own_bernoulli_tape :
-    loc → nat → nat → list (fin 2) → iPropI Σ.
+  Context `{!bernoulli_spec bernoulli}.
   
-  Parameter twp_presample_bernoulli : 
-    ∀ (e : expr) (α : loc) (Φ : val → iProp Σ) 
-      (N M : nat) (ns : list (fin 2)),
-    to_val e = None →
-    own_bernoulli_tape α N M ns ∗ 
-    (∀ i : fin 2, 
-      own_bernoulli_tape α N M (ns ++ [i]) -∗ WP e [{ v, Φ v }]) 
-    ⊢ WP e [{ v, Φ v }].
-  
-  Parameter twp_presample_bernoulli_adv_comp : 
-    ∀ (e : expr) (α : loc) (Φ : val → iProp Σ) 
-      (N M : nat) (ns : list (fin 2)) (ε : R) (D : fin 2 → R),
-    N ≤ M + 1 →
-    (∀ i : fin 2, 0 <= D i) →
-    D 0%fin * (1 - N / (M + 1)) + D 1%fin * (N / (M + 1)) = ε →
-    to_val e = None → 
-    own_bernoulli_tape α N M ns ∗ 
-    ↯ ε ∗ 
-    (∀ i : fin 2, 
-      ↯ (D i) ∗ own_bernoulli_tape α N M (ns ++ [i]) -∗ 
-      WP e [{ v, Φ v }])
-    ⊢ WP e [{ v, Φ v }].
-
-  Parameter twp_bernoulli_tape :
-    ∀ (N M : nat) (α : loc) (ns : list (fin 2)) (n : fin 2),
-    [[{ own_bernoulli_tape α N M (n::ns) }]]
-      bernoulli_tape (#lbl:α) #N #M
-    [[{ RET #n ; own_bernoulli_tape α N M ns }]].
-
-  Parameter twp_presample_bernoulli_planner :
-    ∀ (N M : nat) (e : expr) (ε : nonnegreal) (L : nat) 
-      (α : loc) (Φ : val → iProp Σ) (prefix : list (fin 2)) 
-      (suffix : list (fin 2) → list (fin 2)),
-    (0 < N < S M)%nat →
-    to_val e = None →
-    (∀ junk : list (fin 2), 
-      (0 < length (suffix (prefix ++ junk)) <= L)%nat) → 
-    0 < ε → 
-    ↯ ε ∗ 
-    own_bernoulli_tape α N M prefix ∗
-    ((∃ junk : list (fin 2), 
-      own_bernoulli_tape α N M (prefix ++ junk ++ suffix (prefix ++ junk))) 
-      -∗ WP e [{ v, Φ v }])
-    ⊢ WP e [{ v, Φ v }].
-    
-End BernoulliSpec.
-
-Module BernoulliSpecLemmas (T : BernoulliTapeSpec) (M : BernoulliSpec(T)).
-  Import M.
-
   #[local] Ltac done ::= 
     solve[
       lia |
@@ -99,12 +92,13 @@ Module BernoulliSpecLemmas (T : BernoulliTapeSpec) (M : BernoulliSpec(T)).
       real_solver  |
       tactics.done |
       auto
-    ].
+      ].
+  
   Lemma bernoulli_success_spec (N M : nat) (ε ε' : R) (p := N / S M) :
     (0 <= ε')%R →
     ε = (ε' * (N / S M)) → 
     [[{↯ ε ∗ ↯ (1 - (N / S M))}]]
-      bernoulli #N #M 
+      bernoulli #() #N #M 
     [[{ v, RET v; ↯ ε' ∗ ⌜v = #1⌝ }]].
   Proof.
     iIntros (Hε' ->) "%Φ [Herr Hcost] HΦ".
@@ -118,7 +112,7 @@ Module BernoulliSpecLemmas (T : BernoulliTapeSpec) (M : BernoulliSpec(T)).
 
   Lemma bernoulli_success_spec_simple (N M : nat) :
     [[{↯ (1 - (N / S M))}]]
-      bernoulli #N #M
+      bernoulli #() #N #M
     [[{ v, RET v; ⌜v = #1⌝ }]].
   Proof.
     iIntros (Φ) "Herr HΦ".
@@ -127,12 +121,11 @@ Module BernoulliSpecLemmas (T : BernoulliTapeSpec) (M : BernoulliSpec(T)).
     iApply ("HΦ" with "Hv").
   Qed.
 
-
   Lemma bernoulli_failure_spec (N M : nat) (ε ε' : R) :
     (0 <= ε')%R →
     ε = (ε' * (1 - N / S M)) →
     [[{↯ ε ∗ ↯ (N / S M)}]] 
-      bernoulli #N #M 
+      bernoulli #() #N #M 
     [[{ v, RET v; ↯ ε' ∗ ⌜v = #0⌝ }]].
   Proof.
     iIntros (Hε ->) "%Φ [Herr Hcost] HΦ".
@@ -146,7 +139,7 @@ Module BernoulliSpecLemmas (T : BernoulliTapeSpec) (M : BernoulliSpec(T)).
 
   Lemma bernoulli_failure_spec_simple (N M : nat) :
     [[{↯ (N / S M)}]] 
-      bernoulli #N #M 
+      bernoulli #() #N #M 
     [[{ v, RET v; ⌜v = #0⌝ }]].
   Proof.
     iIntros (Φ) "Herr HΦ".
